hpsim with hsupd

proofmode/HPSim.v
@@ -33,9 +33,7 @@ Section HPSIM.
     fun fmr => forall ctx (WF: URA.wf (fmr ⋅ ctx)),
                exists fmr0, URA.wf (fmr0 ⋅ ctx) /\ P fmr0.
 
-  Hint Unfold hsupd: core.
-
-  Variant __hpsim {with_dummy safe_only: bool}
+  Variant _hpsim'' {with_dummy safe_only: bool}
     (hpsimc hpsimi: forall R (RR: Any.t * R -> Any.t * R -> iProp), bool -> bool -> Any.t * itree hAGEs R -> Any.t * itree hAGEs R -> Σ -> Prop)
     {R} {RR: Any.t * R -> Any.t * R -> iProp}
     : bool -> bool -> Any.t * itree hAGEs R -> Any.t * itree hAGEs R -> Σ -> Prop := 
@@ -43,207 +41,193 @@ Section HPSIM.
       (* Note: (INV: Own fmr ⊢ #=> Ist st_src st_tgt) is required only for the funtion end. *)
       (HPSIM_RET: True)
       ps pt st_src st_tgt fmr v_src v_tgt
-      (K: hsupd (fun fmr0 => Own fmr0 ⊢ RR (st_src,v_src) (st_tgt,v_tgt)) fmr)
+      (K: Own fmr ⊢ RR (st_src,v_src) (st_tgt,v_tgt))
     :
-    __hpsim hpsimc hpsimi ps pt (st_src, Ret v_src) (st_tgt, Ret v_tgt) fmr
+    _hpsim'' hpsimc hpsimi ps pt (st_src, Ret v_src) (st_tgt, Ret v_tgt) fmr
 
   | hpsim_call
       (HPSIM_CALL: True)
       ps pt st_src st_tgt fn varg k_src k_tgt fmr
-      (K: hsupd (fun fmr0 =>
-            exists FR, (Own fmr0 ⊢ (Ist st_src st_tgt ** FR)) /\
-            forall vret st_src0 st_tgt0 fmr' (WF: URA.wf fmr')
-                   (INV: Own fmr' ⊢ (Ist st_src0 st_tgt0 ** FR)),
-            hpsimi R RR true true (st_src0, k_src vret) (st_tgt0, k_tgt vret) fmr') fmr)
+      (K: exists FR, (Own fmr ⊢ (Ist st_src st_tgt ** FR)) /\
+          forall vret st_src0 st_tgt0 fmr' (* (WF: URA.wf fmr') *)
+                 (INV: Own fmr' ⊢ (Ist st_src0 st_tgt0 ** FR)),
+          hpsimi R RR true true (st_src0, k_src vret) (st_tgt0, k_tgt vret) fmr')
     :
-    __hpsim hpsimc hpsimi ps pt (st_src, trigger (Call fn varg) >>= k_src) (st_tgt, trigger (Call fn varg) >>= k_tgt) fmr
+    _hpsim'' hpsimc hpsimi ps pt (st_src, trigger (Call fn varg) >>= k_src) (st_tgt, trigger (Call fn varg) >>= k_tgt) fmr
 
   | hpsim_syscall
       (HPSIM_SYSCALL: True)
       ps pt st_src st_tgt fn varg rvs k_src k_tgt fmr 
-      (K: hsupd (fun fmr0 =>
-            forall vret, 
-            hpsimi R RR true true (st_src, k_src vret) (st_tgt, k_tgt vret) fmr0) fmr)
+      (K: forall vret, 
+          hpsimi R RR true true (st_src, k_src vret) (st_tgt, k_tgt vret) fmr)
     :
-    __hpsim hpsimc hpsimi ps pt (st_src, trigger (Syscall fn varg rvs) >>= k_src) (st_tgt, trigger (Syscall fn varg rvs) >>= k_tgt) fmr
+    _hpsim'' hpsimc hpsimi ps pt (st_src, trigger (Syscall fn varg rvs) >>= k_src) (st_tgt, trigger (Syscall fn varg rvs) >>= k_tgt) fmr
 
   | hpsim_inline_src
       (HPSIM_INLINE_SRC: True)
       (NOTSAFE: negb safe_only)
       ps pt st_src st_tgt fn f varg k_src i_tgt fmr
       (FUN: alist_find fn fl_src = Some f)
-      (K: hsupd (fun fmr0 =>
-            hpsimi R RR true pt (st_src, f varg >>= (if with_dummy then (fun x => trigger (Guarantee True) ;;; trigger (Assume True) ;;; k_src x) else k_src)) (st_tgt, i_tgt) fmr0) fmr)
+      (K: hpsimi R RR true pt (st_src, f varg >>= (if with_dummy then (fun x => trigger (Guarantee True) ;;; trigger (Assume True) ;;; k_src x) else k_src)) (st_tgt, i_tgt) fmr)
     :
-    __hpsim hpsimc hpsimi ps pt (st_src, trigger (Call fn varg) >>= k_src) (st_tgt, i_tgt) fmr
+    _hpsim'' hpsimc hpsimi ps pt (st_src, trigger (Call fn varg) >>= k_src) (st_tgt, i_tgt) fmr
 
   | hpsim_inline_tgt
       (HPSIM_INLINE_TGT: True)
       (NOTSAFE: negb safe_only)
       ps pt st_src st_tgt fn f varg i_src k_tgt fmr
       (FUN: alist_find fn fl_tgt = Some f)
-      (K: hsupd (fun fmr0 =>
-            hpsimi R RR ps true (st_src, i_src) (st_tgt, f varg >>= (if with_dummy then (fun x => trigger (Guarantee True) ;;; trigger (Assume True) ;;; k_tgt x) else k_tgt)) fmr0) fmr)
+      (K: hpsimi R RR ps true (st_src, i_src) (st_tgt, f varg >>= (if with_dummy then (fun x => trigger (Guarantee True) ;;; trigger (Assume True) ;;; k_tgt x) else k_tgt)) fmr)
     :
-    __hpsim hpsimc hpsimi ps pt (st_src, i_src) (st_tgt, trigger (Call fn varg) >>= k_tgt) fmr
+    _hpsim'' hpsimc hpsimi ps pt (st_src, i_src) (st_tgt, trigger (Call fn varg) >>= k_tgt) fmr
 
   | hpsim_tau_src
       (HPSIM_TAU_SRC: True)
       ps pt st_src st_tgt i_src i_tgt fmr
-      (K: hsupd (fun fmr0 =>
-            hpsimi R RR true pt (st_src, i_src) (st_tgt, i_tgt) fmr0) fmr)
+      (K: hpsimi R RR true pt (st_src, i_src) (st_tgt, i_tgt) fmr)
     :
-    __hpsim hpsimc hpsimi ps pt (st_src, tau;; i_src) (st_tgt, i_tgt) fmr
+    _hpsim'' hpsimc hpsimi ps pt (st_src, tau;; i_src) (st_tgt, i_tgt) fmr
 
   | hpsim_tau_tgt
       (HPSIM_TAU_TGT: True)
       ps pt st_src st_tgt i_src i_tgt fmr
-      (K: hsupd (fun fmr0 =>
-            hpsimi R RR ps true (st_src, i_src) (st_tgt, i_tgt) fmr0) fmr)
+      (K: hpsimi R RR ps true (st_src, i_src) (st_tgt, i_tgt) fmr)
     :
-    __hpsim hpsimc hpsimi ps pt (st_src, i_src) (st_tgt, tau;; i_tgt) fmr
+    _hpsim'' hpsimc hpsimi ps pt (st_src, i_src) (st_tgt, tau;; i_tgt) fmr
 
   | hpsim_take_src
       (HPSIM_TAKE_SRC: True)
       ps pt st_src st_tgt X k_src i_tgt fmr
-      (K: hsupd (fun fmr0 =>
-            forall (x: X), hpsimi R RR true pt (st_src, k_src x) (st_tgt, i_tgt) fmr0) fmr)
+      (K: forall (x: X), hpsimi R RR true pt (st_src, k_src x) (st_tgt, i_tgt) fmr)
     :
-    __hpsim hpsimc hpsimi ps pt (st_src, trigger (Take X) >>= k_src) (st_tgt, i_tgt) fmr
+    _hpsim'' hpsimc hpsimi ps pt (st_src, trigger (Take X) >>= k_src) (st_tgt, i_tgt) fmr
 
   | hpsim_choose_tgt
       (HPSIM_CHOOSE_TGT: True)
       ps pt st_src st_tgt X i_src k_tgt fmr
-      (K: hsupd (fun fmr0 =>
-            forall (x: X), hpsimi R RR ps true (st_src, i_src) (st_tgt, k_tgt x) fmr0) fmr)
+      (K: forall (x: X), hpsimi R RR ps true (st_src, i_src) (st_tgt, k_tgt x) fmr)
     :
-    __hpsim hpsimc hpsimi ps pt (st_src, i_src) (st_tgt, trigger (Choose X) >>= k_tgt) fmr
+    _hpsim'' hpsimc hpsimi ps pt (st_src, i_src) (st_tgt, trigger (Choose X) >>= k_tgt) fmr
 
   | hpsim_choose_src
       (HPSIM_CHOOSE_SRC: True)
       (NOTSAFE: negb safe_only)
       ps pt st_src st_tgt X k_src i_tgt fmr
-      (K: hsupd (fun fmr0 =>
-            exists x, hpsimi R RR true pt (st_src, k_src x) (st_tgt, i_tgt) fmr0) fmr)
+      (K: exists x, hpsimi R RR true pt (st_src, k_src x) (st_tgt, i_tgt) fmr)
     :
-    __hpsim hpsimc hpsimi ps pt (st_src, trigger (Choose X) >>= k_src) (st_tgt, i_tgt) fmr
+    _hpsim'' hpsimc hpsimi ps pt (st_src, trigger (Choose X) >>= k_src) (st_tgt, i_tgt) fmr
 
   | hpsim_take_tgt
       (HPSIM_TAKE_TGT: True)
       (NOTSAFE: negb safe_only)
       ps pt st_src st_tgt X i_src k_tgt fmr
-      (K: hsupd (fun fmr0 =>
-            exists x, hpsimi R RR ps true (st_src, i_src) (st_tgt, k_tgt x) fmr0) fmr)
+      (K: exists x, hpsimi R RR ps true (st_src, i_src) (st_tgt, k_tgt x) fmr)
     :
-    __hpsim hpsimc hpsimi ps pt (st_src, i_src) (st_tgt, trigger (Take X) >>= k_tgt) fmr
+    _hpsim'' hpsimc hpsimi ps pt (st_src, i_src) (st_tgt, trigger (Take X) >>= k_tgt) fmr
 
   | hpsim_supdate_src
       (HPSIM_SUPDATE_SRC: True)
       ps pt st_src st_tgt X (run: Any.t -> Any.t * X) st_src0 x k_src i_tgt fmr
       (RUN: run st_src = (st_src0, x))      
-      (K: hsupd (fun fmr0 =>
-            hpsimi R RR true pt (st_src0, k_src x) (st_tgt, i_tgt) fmr0) fmr)
+      (K: hpsimi R RR true pt (st_src0, k_src x) (st_tgt, i_tgt) fmr)
     :
-    __hpsim hpsimc hpsimi ps pt (st_src, trigger (SUpdate run) >>= k_src) (st_tgt, i_tgt) fmr
+    _hpsim'' hpsimc hpsimi ps pt (st_src, trigger (SUpdate run) >>= k_src) (st_tgt, i_tgt) fmr
 
   | hpsim_supdate_tgt
       (HPSIM_SUPDATE_TGT: True)
       ps pt st_src st_tgt X (run: Any.t -> Any.t * X) st_tgt0 x i_src k_tgt fmr
       (RUN: run st_tgt = (st_tgt0, x))
-      (K: hsupd (fun fmr0 =>
-            hpsimi R RR ps true (st_src, i_src) (st_tgt0, k_tgt x) fmr0) fmr)
+      (K: hpsimi R RR ps true (st_src, i_src) (st_tgt0, k_tgt x) fmr)
     :
-    __hpsim hpsimc hpsimi ps pt (st_src, i_src) (st_tgt, trigger (SUpdate run) >>= k_tgt) fmr
+    _hpsim'' hpsimc hpsimi ps pt (st_src, i_src) (st_tgt, trigger (SUpdate run) >>= k_tgt) fmr
 
   | hpsim_assume_src
       (HPSIM_ASSUME_SRC: True)
       ps pt st_src st_tgt iP k_src i_tgt fmr
-      (K: hsupd (fun fmr0 =>
-            forall fmr' (WF: URA.wf fmr')
-                   (NEW: Own fmr' ⊢ (iP ** Own fmr0)),
-            hpsimi R RR true pt (st_src, k_src tt) (st_tgt, i_tgt) fmr') fmr)
+      (K: forall fmr' (* (WF: URA.wf fmr') *)
+                 (NEW: Own fmr' ⊢ (iP ** Own fmr)),
+          hpsimi R RR true pt (st_src, k_src tt) (st_tgt, i_tgt) fmr')
     :
-    __hpsim hpsimc hpsimi ps pt (st_src, trigger (Assume iP) >>= k_src) (st_tgt, i_tgt) fmr
+    _hpsim'' hpsimc hpsimi ps pt (st_src, trigger (Assume iP) >>= k_src) (st_tgt, i_tgt) fmr
 
   | hpsim_guarantee_tgt
       (HPSIM_GUARANTEE_TGT: True)
       ps pt st_src st_tgt iP i_src k_tgt fmr
-      (K: hsupd (fun fmr0 =>
-            forall fmr' (WF: URA.wf fmr')
-                   (NEW: Own fmr' ⊢ (iP ** Own fmr0)),
-            hpsimi R RR ps true (st_src, i_src) (st_tgt, k_tgt tt) fmr') fmr)
+      (K: forall fmr' (* (WF: URA.wf fmr') *)
+                 (NEW: Own fmr' ⊢ (iP ** Own fmr)),
+          hpsimi R RR ps true (st_src, i_src) (st_tgt, k_tgt tt) fmr')
     :
-    __hpsim hpsimc hpsimi ps pt (st_src, i_src) (st_tgt, trigger (Guarantee iP) >>= k_tgt) fmr
+    _hpsim'' hpsimc hpsimi ps pt (st_src, i_src) (st_tgt, trigger (Guarantee iP) >>= k_tgt) fmr
 
   | hpsim_guarantee_src
       (HPSIM_GUARANTEE_SRC: True)
       (NOTSAFE: negb safe_only)
       ps pt st_src st_tgt iP k_src i_tgt fmr 
-      (K: hsupd (fun fmr0 =>
-            exists FMR, (Own fmr0 ⊢ iP ** FMR) /\
-            forall fmr' (WF: URA.wf fmr')
-                   (NEW: Own fmr' ⊢ FMR),
-              hpsimi R RR true pt (st_src, k_src tt) (st_tgt, i_tgt) fmr') fmr)
+      (K: exists FMR, (Own fmr ⊢ iP ** FMR) /\
+          forall fmr' (* (WF: URA.wf fmr') *)
+                 (NEW: Own fmr' ⊢ FMR),
+            hpsimi R RR true pt (st_src, k_src tt) (st_tgt, i_tgt) fmr')
     :
-    __hpsim hpsimc hpsimi ps pt (st_src, trigger (Guarantee iP) >>= k_src) (st_tgt, i_tgt) fmr
+    _hpsim'' hpsimc hpsimi ps pt (st_src, trigger (Guarantee iP) >>= k_src) (st_tgt, i_tgt) fmr
 
   | hpsim_assume_tgt
       (HPSIM_ASSUME_TGT: True)
       (NOTSAFE: negb safe_only)
       ps pt st_src st_tgt iP i_src k_tgt fmr 
-      (K: hsupd (fun fmr0 =>
-            exists FMR, (Own fmr0 ⊢ iP ** FMR) /\
-            forall fmr' (WF: URA.wf fmr')
-                   (NEW: Own fmr' ⊢ FMR),
-            hpsimi R RR ps true (st_src, i_src) (st_tgt, k_tgt tt) fmr') fmr)
+      (K: exists FMR, (Own fmr ⊢ iP ** FMR) /\
+          forall fmr' (* (WF: URA.wf fmr') *)
+                 (NEW: Own fmr' ⊢ FMR),
+          hpsimi R RR ps true (st_src, i_src) (st_tgt, k_tgt tt) fmr')
     :
-    __hpsim hpsimc hpsimi ps pt (st_src, i_src) (st_tgt, trigger (Assume iP) >>= k_tgt) fmr
+    _hpsim'' hpsimc hpsimi ps pt (st_src, i_src) (st_tgt, trigger (Assume iP) >>= k_tgt) fmr
 
   | hpsim_progress
       (HPSIM_PROGRESS: True)
       (NOTSAFE: negb safe_only)
       sti_src sti_tgt fmr
-      (K: hsupd (fun fmr0 =>
-              hpsimc R RR false false sti_src sti_tgt fmr0) fmr)
+      (K: hpsimc R RR false false sti_src sti_tgt fmr)
     :
-    __hpsim hpsimc hpsimi true true sti_src sti_tgt fmr
+    _hpsim'' hpsimc hpsimi true true sti_src sti_tgt fmr
   .
-  Arguments __hpsim with_dummy safe_only hpsimc hpsimi R RR.
+  Arguments _hpsim'' with_dummy safe_only hpsimc hpsimi R RR.
+
+  Definition _hpsim' with_dummy safe_only hpsimc hpsimi R RR ps pt sti_src sti_tgt :=
+    hsupd (@_hpsim'' with_dummy safe_only hpsimc hpsimi R RR ps pt sti_src sti_tgt).
 
   Inductive _hpsim {with_dummy} hpsim R RR ps pt sti_src sti_tgt fmr : Prop
     :=
-  | hpsimF_intro (IN: @__hpsim with_dummy false hpsim (@_hpsim with_dummy hpsim) R RR ps pt sti_src sti_tgt fmr) 
+  | hpsimF_intro (IN: @_hpsim' with_dummy false hpsim (@_hpsim with_dummy hpsim) R RR ps pt sti_src sti_tgt fmr) 
   .
   
   Definition hpsim {R} RR := paco7 (@_hpsim false) bot7 R RR.
 
   Lemma _hpsim_tarski with_dummy hpsim rel
-    (FIX: @__hpsim with_dummy false hpsim rel <7= rel)
+    (FIX: @_hpsim' with_dummy false hpsim rel <7= rel)
     :
     @_hpsim with_dummy hpsim <7= rel.
   Proof.
     fix self 8. i.
     destruct PR. apply FIX.
-    destruct IN; econs; unfold hsupd in *; ss; eauto;
-      try by i; exploit K; eauto; i; des; esplits; eauto.
+    ii. exploit IN; eauto. i; des.
+    destruct x8; des; esplits; eauto; econs; esplits; eauto.
   Qed.
 
-  Lemma __hpsim_mon with_dummy safe_only r r' R RR s s'
+  Lemma _hpsim'_mon with_dummy safe_only r r' R RR s s'
     ps pt sti_src sti_tgt fmr
-    (REL: @__hpsim with_dummy safe_only r s R RR ps pt sti_src sti_tgt fmr)
+    (REL: @_hpsim' with_dummy safe_only r s R RR ps pt sti_src sti_tgt fmr)
     (LEr: r <7= r')
     (LEs: s <7= s')
     :
-    @__hpsim with_dummy safe_only r' s' R RR ps pt sti_src sti_tgt fmr.
+    @_hpsim' with_dummy safe_only r' s' R RR ps pt sti_src sti_tgt fmr.
   Proof.
-    ii. destruct REL; econs; unfold hsupd in *; eauto;
-      try by i; exploit K; eauto; i; des; esplits; eauto.
+    ii. exploit REL; eauto. i; des.
+    destruct x1; des; esplits; eauto; econs; esplits; eauto.
   Qed.
 
   Lemma _hpsim_mon with_dummy: monotone7 (@_hpsim with_dummy).
   Proof. 
     ii. eapply _hpsim_tarski, IN.
-    i. econs. eapply __hpsim_mon; eauto.
+    i. econs. eapply _hpsim'_mon; eauto.
   Qed.
 
   Lemma _hpsim_mon_auto with_dummy r r' R RR
@@ -254,9 +238,9 @@ Section HPSIM.
     @_hpsim with_dummy r' R RR ps pt sti_src sti_tgt fmr.
   Proof. eapply _hpsim_mon; eauto. Qed.
   
-  Hint Constructors __hpsim _hpsim.
-  Hint Unfold hpsim.
-  Hint Resolve __hpsim_mon: paco.
+  Hint Constructors _hpsim'' _hpsim.
+  Hint Unfold _hpsim' hpsim.
+  Hint Resolve _hpsim'_mon: paco.
   Hint Resolve _hpsim_mon: paco.
   Hint Resolve _hpsim_mon_auto: paco.
   Hint Resolve cpn7_wcompat: paco.
@@ -268,7 +252,7 @@ Section HPSIM.
   Definition hpsim_body := @hpsim Any.t hpsim_tail.
 
   Definition hpsim_fun (i_src: itree hAGEs Any.t) (i_tgt: itree hAGEs Any.t):  Prop :=
-    forall st_src st_tgt fmr (WF: URA.wf fmr)
+    forall st_src st_tgt fmr (* (WF: URA.wf fmr) *)
            (INV: Own fmr ⊢ Ist st_src st_tgt),
       hpsim_body false false (st_src, i_src) (st_tgt, i_tgt) fmr.
 
@@ -296,31 +280,40 @@ Section HPSIM.
       repeat f_equal. extensionality x. rewrite bind_ret_l. eauto.
   Qed.
 
-  Lemma __hpsim_upd
-    with_dummy safe_only hpsimc hpsimi R RR ps pt sti_src sti_tgt (fmr: Σ)
-    (WF: URA.wf fmr)
-    (K: hsupd (@__hpsim with_dummy safe_only hpsimc hpsimi R RR ps pt sti_src sti_tgt) fmr)
+  Lemma hsupd_mon P Q
+    (LE: P <1= Q)
     :
-    @__hpsim with_dummy safe_only hpsimc hpsimi R RR ps pt sti_src sti_tgt fmr.
+    hsupd P <1= hsupd Q.
   Proof.
-    r in K. exploit (K ε); r_solve; i; des; eauto.
-    destruct x1.
-    - 
-      
-    econs; eauto; r; i. 
-exploit K; eauto. i; des. 
+    unfold hsupd; i. exploit PR; eauto.
+    i; des. esplits; eauto.
+  Qed.
 
-
-depdes x2; unfold hsupd in *; try by exploit K1; eauto.
-
-
- 
-  esplits; eauto with paco.
-
-    
-    try by econs; eauto; r; i; exploit K; eauto; i; des; esplits; eauto with paco.
+  Lemma hsupd_incl P
+    :
+    P <1= hsupd P.
+  Proof.
+    unfold hsupd; i. esplits; eauto.
   Qed.
   
+  Lemma hsupd_merge P r
+    (REL: hsupd (hsupd P) r)
+    :
+    hsupd P r.
+  Proof.
+    unfold hsupd in *. i. specialize (REL ctx WF). des.
+    specialize (REL0 _ REL). des. eauto.
+  Qed.
+  
+  Lemma _hpsim'_upd
+    with_dummy safe_only hpsimc hpsimi R RR ps pt sti_src sti_tgt (fmr: Σ)
+    (K: hsupd (@_hpsim' with_dummy safe_only hpsimc hpsimi R RR ps pt sti_src sti_tgt) fmr)
+    :
+    @_hpsim' with_dummy safe_only hpsimc hpsimi R RR ps pt sti_src sti_tgt fmr.
+  Proof.
+    eapply hsupd_merge. eauto.
+  Qed.
+
   Lemma _hpsim_flag_mon r R RR (ps pt ps' pt': bool) st_src st_tgt fmr
     (SIM: @_hpsim false r R RR ps pt st_src st_tgt fmr)
     (LES: ps -> ps')
@@ -331,10 +324,11 @@ depdes x2; unfold hsupd in *; try by exploit K1; eauto.
     move SIM before r. revert_until SIM.
     pattern R, RR, ps, pt, st_src, st_tgt, fmr.
     eapply _hpsim_tarski, SIM. i. econs.
-    destruct PR; ss; eauto with paco;
-      try by econs; unfold hsupd in *; i; eauto; exploit K; eauto; i; des; esplits; eauto with paco.
+    ii. exploit PR; eauto. i; des.
+    destruct x8; des; esplits; eauto; try by econs; esplits; eauto.
     hexploit LES; eauto; i. hexploit LET; eauto; i.
-    destruct ps', pt'; clarify. eauto with paco.
+    destruct ps', pt'; try discriminate. 
+    econs; esplits; eauto.
   Qed.
 
   Lemma hpsim_flag_mon R RR (ps pt ps' pt': bool) st_src st_tgt fmr
@@ -354,7 +348,7 @@ depdes x2; unfold hsupd in *; try by exploit K1; eauto.
     :
     gpaco7 (@_hpsim with_dummy) (cpn7 (@_hpsim with_dummy)) r g R RR true true st_src st_tgt fmr.
   Proof.
-    gstep. eauto 10.
+    gstep. econs. econs; eauto.
   Qed.
 
 
@@ -385,10 +379,10 @@ depdes x2; unfold hsupd in *; try by exploit K1; eauto.
     eapply GF in SIM.
     move SIM before GF. revert_until SIM. pattern x0, x1, ps0, pt0, x4, x5, x6.
     eapply _hpsim_tarski, SIM. econs.
-    destruct PR; clarify; et;
-      try by econs; et; rr; i; exploit K; eauto; i; des; esplits; eauto with paco.
+    ii. exploit PR; eauto. i; des.
+    destruct x15; des; esplits; eauto; try by econs; esplits; eauto.
     exploit SRC; et. exploit TGT; et. i; clarify.
-    econs; et; rr; i; exploit K; eauto; i; des; esplits; eauto with paco.
+    econs; esplits; eauto using rclo7.
   Qed.
 
   Lemma hpsim_flag_down with_dummy R RR r g ps pt st_src st_tgt fmr
@@ -403,33 +397,36 @@ depdes x2; unfold hsupd in *; try by exploit K1; eauto.
 
 
   Definition hpsimC with_dummy hpsim :=
-    @__hpsim with_dummy false hpsim hpsim.
+    @_hpsim' with_dummy false hpsim hpsim.
   
   Lemma hpsimC_mon with_dummy : monotone7 (@hpsimC with_dummy).
   Proof.
-    ii. inv IN; econs; eauto;
-      try by rr; i; exploit K; eauto; i; des; esplits; eauto with paco.
+    ii. exploit IN; eauto. i; des.
+    destruct x8; des; esplits; eauto; try by econs; esplits; eauto.
   Qed.
 
   Lemma hpsimC_spec with_dummy:
     (@hpsimC with_dummy) <8= gupaco7 (@_hpsim with_dummy) (cpn7 (@_hpsim with_dummy)).
   Proof.
     eapply wrespect7_uclo; eauto with paco.
-    econs; eauto using hpsimC_mon; i. econs.
-    inv PR; econs; i; et; try (eapply _hpsim_mon; eauto using rclo7);
-      try by rr; i; exploit K; eauto; i; des; esplits; eauto with paco.
+    econs; eauto using hpsimC_mon; i.
+    econs. ii. exploit PR; eauto. i; des.
+    destruct x8; des; esplits; eauto;
+      try by econs; esplits; eauto; i; try eapply _hpsim_mon; eauto using rclo7.
   Qed.
   
 
 
 
   Definition safe_hpsim hpsim :=
-    @__hpsim false true hpsim hpsim.
+    @_hpsim' false true hpsim hpsim.
 
   Lemma safe_hpsim_spec:
     safe_hpsim <8= gupaco7 (@_hpsim false) (cpn7 (@_hpsim false)).
   Proof.
-    i. eapply hpsimC_spec. depdes PR; try by (econs; et).
+    i. eapply hpsimC_spec. ii. exploit PR; eauto.
+    i; des. esplits; eauto.
+    destruct x9; econs; eauto.
   Qed.
 
 
@@ -469,21 +466,20 @@ depdes x2; unfold hsupd in *; try by exploit K1; eauto.
     remember (st_src, i_src) as sti_src. remember (st_tgt, i_tgt) as sti_tgt.
     move SIM before GF. revert_until SIM.
     pattern Q, QQ, ps, pt, sti_src, sti_tgt, fmr.
-    eapply _hpsim_tarski, SIM. econs.
-    destruct PR; i; depdes Heqsti_src Heqsti_tgt; grind; eauto with paco;
-      try by econs; rr; i; eauto; exploit K; eauto; i; des; esplits; eauto with paco.
-    - rr in K.
-
-
-      hexploit SIMK; eauto.
-      { r in K.
-      i.
-      apply GF in H. eapply _hpsim_mon; cycle 1.
-      { i. econs. apply PR. }
-      eapply _hpsim_flag_mon; eauto; clarify.
-    - econs; eauto. rewrite <-!bind_bind. eapply K; eauto.
-    - econs; eauto. rewrite <-!bind_bind. eapply K; eauto.
-    - econs; eauto. eauto 10 using rclo7, hpsim_bindC.
+    eapply _hpsim_tarski, SIM. econs. apply _hpsim'_upd.
+    ii. exploit PR; eauto. i; des.
+    destruct x8; des; depdes Heqsti_src Heqsti_tgt; grind; esplits;
+      try by ii; esplits; eauto with paco.
+    - hexploit SIMK; eauto. i. apply GF in H.
+      eapply _hpsim_mon.
+      { eapply _hpsim_flag_mon; eauto; i; clarify. }
+      eauto using rclo7.
+    - do 2 (econs; esplits; eauto).
+      rewrite <-!bind_bind. eapply K; eauto.
+    - do 2 (econs; esplits; eauto).
+      rewrite <-!bind_bind. eapply K; eauto.
+    - do 2 (econs; esplits; eauto).
+      eauto 10 using rclo7, hpsim_bindC.
   Qed.
 
   Lemma hpsim_bindC_spec:
@@ -540,9 +536,10 @@ depdes x2; unfold hsupd in *; try by exploit K1; eauto.
     intros. destruct PR. move SIM before r. revert_until SIM.
     pattern R, RR, ps, pt, sti_src, sti_tgt, fmr.
     eapply _hpsim_tarski, SIM. econs.
-    destruct PR; econs; eauto using hpsim_extendC;
-      try by i; exploit K; eauto using URA_wf_extends_add; i; des; esplits; eauto using URA_extends_refl.
-    etrans; try eassumption. eapply Own_extends; eauto.
+    ii. exploit PR; eauto using URA_wf_extends_add. i; des.
+    destruct x8; des; grind; esplits; eauto using hpsim_extendC, URA_extends_refl;
+      econs; rr; esplits; i; eauto;
+      try by try eapply K; try eapply K0; eauto; try refl.
   Qed.
   
   Lemma hpsim_extendC_spec:
@@ -560,9 +557,8 @@ depdes x2; unfold hsupd in *; try by exploit K1; eauto.
     forall R (RR: Any.t * R -> Any.t * R -> iProp), bool -> bool -> Any.t * itree hAGEs R -> Any.t * itree hAGEs R -> Σ -> Prop
   :=
   | hpsim_updateC_intro
-      ps pt R RR sti_src sti_tgt fmr (WF: URA.wf fmr)
-      (EXT: forall ctx (WF: URA.wf (fmr ⋅ ctx)),
-            exists fmr0, r R RR ps pt sti_src sti_tgt fmr0)
+      ps pt R RR sti_src sti_tgt fmr
+      (EXT: hsupd (r R RR ps pt sti_src sti_tgt) fmr)
      :
     hpsim_updateC r R RR ps pt sti_src sti_tgt fmr
   .
@@ -574,26 +570,19 @@ depdes x2; unfold hsupd in *; try by exploit K1; eauto.
     hpsim_updateC r1 <7= hpsim_updateC r2
   .
   Proof.
-    ii. destruct PR. econs; eauto. i. exploit EXT; i; des; eauto.
+    ii. destruct PR. econs; eauto.
+    ii. exploit EXT; i; des; eauto.
   Qed.
 
   Lemma hpsim_updateC_compatible:
     compatible7 (@_hpsim false) hpsim_updateC.
   Proof.
     econs; eauto using hpsim_updateC_mon.
-    intros. destruct PR. exploit (EXT ε).
-    { r_solve. eauto. }
-    i. destruct x0 as [fmr0 SIM].
-    move SIM before r. revert_until SIM.
-    pattern R, RR, ps, pt, sti_src, sti_tgt, fmr0.
-    eapply _hpsim_tarski, SIM. econs.
-    destruct PR; econs; eauto using hpsim_updateC.
-Focus 2.
-  i; exploit K; eauto.
-
-    
-      try by i; exploit K; eauto using URA_wf_extends_add; i; des; esplits; eauto using URA_extends_refl.
-    etrans; try eassumption. eapply Own_extends; eauto.
+    i. destruct PR. econs. eapply _hpsim'_upd.
+    eapply hsupd_mon, EXT.
+    i. destruct PR.
+    eapply _hpsim'_mon; eauto using hpsim_updateC, hsupd_incl.
+    i. eapply _hpsim_mon; eauto using hpsim_updateC, hsupd_incl.
   Qed.
   
   Lemma hpsim_updateC_spec:
@@ -921,23 +910,32 @@ Hint Resolve cpn7_wcompat: paco.
 (**********)
 
 Lemma hpsim_refl {Σ: GRA.t} fl:
-  forall st itr fmr (WF: URA.wf fmr),
-  hpsim_body fl fl (fun src tgt => ⌜src = tgt⌝%I) false false (st, itr) (st, itr) fmr.
+  forall src tgt fmr (EQST: Own fmr ⊢ ⌜src = tgt⌝%I),
+  hpsim_body fl fl (fun src tgt => ⌜src = tgt⌝%I) false false src tgt fmr.
 Proof.
   ginit. gcofix CIH. i.
-  gstep. econs. assert (CASE := case_itrH _ itr); des; subst.
-  - repeat (econs; eauto with paco).
-  - repeat (econs; eauto with paco).
-  - repeat (econs; eauto with paco).
-  - repeat (econs; eauto with paco).
-  - destruct c; econs; eauto.
-    i. exists fmr, (Own fmr); esplits; eauto.
-    do 2 econs; eauto.
-    uipropall. exploit INV; i; eauto; try refl.
-    des. rr in x1. uipropall. subst. eauto with paco.
+  destruct (classic (URA.wf fmr)); cycle 1.
+  { gstep. econs. econs. exfalso. apply H. eapply URA.wf_mon; eauto. }
+  assert (src = tgt); subst.
+  { rr in EQST. uiprop in EQST. rr in EQST. uiprop in EQST.
+    eapply EQST; eauto; refl. }
+
+  destruct tgt as [st itr].
+  gstep. econs. econs. assert (CASE := case_itrH _ itr); des; subst;
+    try by repeat (econs; eauto with paco).
+  - esplits; eauto. destruct c; econs; eauto.
+    exists (Own fmr). esplits; eauto.
+    i. do 2 econs; esplits; eauto.
+    assert (st_src0 = st_tgt0); subst.
+    { uipropall. exploit INV; i; des; try refl; eauto.
+      - eapply URA.wf_mon; eauto.
+      - rr in x1. uipropall.
+    }
+    econs; eauto with paco.
   - depdes s; destruct (run st) eqn: EQ.
     repeat (econs; eauto with paco).
   - depdes e; repeat (econs; eauto with paco).
+Unshelve. eauto.
 Qed.
 
 (**********)
@@ -970,8 +968,9 @@ Proof.
     generalize (HModSem.fnsems ms).
     induction a; ii; ss.
     econs; et. econs; ss. ii; clarify.
-    eapply own_pure in INV; eauto; cycle 1.
-    subst. eapply hpsim_refl; eauto.
+    eapply hpsim_refl; eauto.
+    iIntros "H". iPoseProof (INV with "H") as "H". iStopProof.
+    rr. uipropall. i. rr in H. rr. uipropall. subst. eauto.
   - iIntros "H". eauto.
 Qed.
 
